Rename files

src/code.lean
@@ -1,247 +1,117 @@
-import computability.turing_machine
 import computability.partrec
-import boolcodeable
+import computability.encoding
+import pair
 import part
 
-/-- If you fold a list using `bind` and you encounter `none` at any point, the result will be `none` -/
-@[simp] lemma foldl_bind_part_none {α β : Type*} (f : α → β → part α) (ls : list β) :
-  ls.foldl (λ (a : part α) (hd : β), a.bind (λ a', f a' hd)) part.none = part.none :=
-by { induction ls with hd tl ih, { refl, }, simpa, }
+open computability (encode_nat decode_nat)
 
 section
 parameter (ι : Type)
 
-local attribute [reducible] bitstring
-
-/-- The current implementation has all the "starting functions" that `code` starts out with
-into `oracle`. The oracles have type `ι`.
-
-The spec for `code` is basically the same as `to_partrec.code`
-
-TODO: decide if this is a good design decision or if all the oracles
-should just be moved into `code` explicitly. Maybe `code`'s with oracles can be created at a future date. -/
 inductive code
-| oracle : ι →  code
+| fst : code
+| snd : code
+| bit : bool → code
 | pair : code → code → code
 | comp : code → code → code
-| case : code → code → code
+| case : code → code → code → code
 | fix : code → code
 
 parameter {ι}
 /-- Given an implementation `impl` of the oracles, we can evaluate the `code`. -/
-@[simp] def code.eval (impl : ι → bitstring → bitstring) : code → bitstring →. bitstring
-| (code.oracle i) := λ v, pure (impl i v)
-| (code.pair f g) := λ v, do x ← f.eval v, y ← g.eval v, return (boolcodeable.encode (x, y)) 
+@[simp] def code.eval : code → ℕ →. ℕ
+| code.fst := λ n, part.some (nat.unpair' n).1
+| code.snd := λ n, part.some (nat.unpair' n).2
+| (code.bit b) := nat.bit b
+| (code.pair f g) := λ v, do x ← f.eval v, y ← g.eval v, return (nat.mkpair' x y) 
 | (code.comp f g) := λ v, g.eval v >>= f.eval
-| (code.case f g) := λ v, if v.head = ff then f.eval v.tail else g.eval v.tail
+| (code.case f g h) := λ v, match encode_nat v with
+  | [] := h.eval 0
+  | (ff :: xs) := f.eval (decode_nat xs)
+  | (tt :: xs) := g.eval (decode_nat xs)
+end
 | (code.fix f) := pfun.fix $ λ v, (f.eval v).map $ λ v',
-  if v'.head = ff then sum.inl v'.tail else sum.inr v'.tail
-
--- TODO: add code.eval_tree which evaluates without `impl` (or maybe a partial `impl`), and returns
--- a (possibly infinite) binary tree consisting of all the possible outputs based on the results of the oracle.
-
-/-
-Description of oracles:
-  - `fst` -- decodes a tuple `(a, b)` and returns `a`
-  - `snd` -- decodes a tuple `(a, b)` and returns `b`
-  - `head` -- returns the first bit. Note that this does NOT return the first element of an encoded list. 
-  - `tail` -- returns all but the first bit
-  - `append` -- concatentates two bitstrings
-  - `ff'` -- returns the constant `ff` bit
-  - `tt'` -- returns the constant `tt'` bit
-  - `isempty` -- returns `[ff]` or `[tt]` based on if the input is `0` bits long
-  - `id` -- returns the bitstring unchanged
-  - `add` -- adds two encodings of natural numbers
-  - `sum` -- subtracts two encodings of natural numbers
-  - `mul` -- multiplies two encodings of natural numbers 
-
-Note that all of these are not necessary
-For example, `fst`, `snd`, `append`, `ff'`, `tt'`, `isempty` should be enough, if we change the
-implementation of `ff'` and `tt'` to cons instead of returns a constant bitstring.
-
-In particular, the implementations could be something like (pseudocode):
-  - `nil = fst (tt :: input)` (i.e. `fst ∘ tt'`)
-  - `id = snd (tt :: input)`
-  - `head = fst (ff :: tt :: input)`
-  - `tail = snd (ff :: tt :: input)`
-
-However, these depend on the implementation details of the encoding of tuples. I'm adding more here
-just for convenience for now, and so that it's easier to change that encoding if need be,
-but when we compile to TM's, we will want to remove some.
--/
-inductive ocl
-| fst | snd | head | tail | append | isempty | id
-| ff' | tt'
-| add | mul | sub
-
-
-@[simp] def impl : ocl → bitstring → bitstring
-| ocl.fst := λ x, (boolcodeable.decode_tuple x).1
-| ocl.snd := λ x, (boolcodeable.decode_tuple x).2
-| ocl.ff' := λ _, [ff]
-| ocl.tt' := λ _, [tt]
-| ocl.head := λ x, [x.head]
-| ocl.tail := list.tail
-| ocl.isempty := λ x, [x.empty]
-| ocl.id := λ x, x
-| ocl.append := λ x, function.uncurry list.append (boolcodeable.decode _ x).iget
-| ocl.add := λ x, boolcodeable.encode (function.uncurry nat.add (boolcodeable.decode _ x).iget)
-| ocl.mul := λ x, boolcodeable.encode (function.uncurry nat.mul (boolcodeable.decode _ x).iget)
-| ocl.sub := λ x, boolcodeable.encode (function.uncurry nat.sub (boolcodeable.decode _ x).iget)
+  if (nat.unpair' v').1 = 0 then sum.inl (nat.unpair' v').2 else sum.inr (nat.unpair' v').2
 
 end
 
 section
-/-! Here, we define lots of misc. functions that will be useful, culminating with an implementation of
-  `list.foldl`. Given that, we should be able to implement everything else useful. -/
-open ocl code boolcodeable (encode decode encode_tuple decode_tuple)
-
-local attribute [reducible] bitstring
-
--- TODO: choose better notation
-local notation f `ᵒ`:10000 := oracle f
+open code
 local notation `{` x `, ` y `}` := pair x y
 infixr `∘`:90 := comp
 
--- Just testing some lemmas
-def append' (f g : code ocl) : code ocl := appendᵒ ∘ {f, g}
-@[simp] lemma append'_apply (f g : code ocl) (bs : bitstring) :
-  (append' f g).eval impl bs = (do x ← f.eval impl bs, y ← g.eval impl bs, return (x ++ y)) :=
+def zero : code := fst ∘ (bit tt)
+@[simp] lemma zero_apply (n : ℕ) : zero.eval n = part.some 0 :=
+by simp [zero, nat.bit, ← nat.mkpair'_zero]
+
+def one : code := bit tt ∘ zero
+@[simp] lemma one_apply (n : ℕ) : one.eval n = part.some 1 :=
+by simp [one, nat.bit]
+
+protected def code.id : code := snd ∘ (bit tt)
+@[simp] lemma id_apply (n : ℕ) : code.id.eval n = part.some n :=
+by simp [code.id, nat.bit, ← nat.mkpair'_zero]
+
+def append_const : list bool → code
+| [] := code.id
+| (b :: bs) := bit b ∘ (append_const bs)
+lemma append_const_apply (bs : list bool) (n : ℕ) :
+  (append_const bs).eval n = part.some (bs.foldr nat.bit n) :=
+by { induction bs with _ _ ih, { simp [append_const], }, simp [append_const, ih], }
+lemma append_const_apply' (bs : list bool) (n : ℕ) (hn : n ≠ 0 ∨ bs.last'.get_or_else tt = tt) :
+  (append_const bs).eval n = part.some (decode_nat (bs ++ encode_nat n)) :=
+by { cases hn, rw [append_const_apply, computability.append_bits _ hn], rw [append_const_apply, computability.append_bits' _ hn], }
+
+protected def code.const (c : ℕ) : code := (append_const (encode_nat c)) ∘ zero
+@[simp] lemma const_apply (c n : ℕ) : (code.const c).eval n = part.some c :=
 begin
-  simp only [append', code.eval],
-  -- TODO: extract to tactic (e.g. `assume_halts`)
-  -- Also this uses LEM. I don't feel bad about it. But we really need a good
-  -- tactic that helps break `part`'s into cases, because they are annoying to work with right now.
-  cases (f.eval impl bs) with d₁ v₁, by_cases h₁ : d₁, swap, { simp [h₁], }, simp only [h₁, part.mk_some],
-  cases (g.eval impl bs) with d₂ v₂, by_cases h₂ : d₂, swap, { simp [h₂], }, simp only [h₂, part.mk_some],
-  simp, refl,
+  simp only [code.const, code.eval, zero_apply, part.bind_eq_bind, part.bind_some],
+  rw append_const_apply', { simp, },
+  right, simp,
 end
 
-def nil : code ocl := tailᵒ ∘ ff'ᵒ
-@[simp] lemma nil_apply (bs : bitstring) : nil.eval impl bs = part.some [] := by simp [nil]
-
-def cons (f g : code ocl) : code ocl := appendᵒ ∘ {headᵒ ∘ f, g}
-@[simp] lemma cons_apply (f g : code ocl) (bs : bitstring) :
-  (cons f g).eval impl bs = (do x ← f.eval impl bs, y ← g.eval impl bs, return (x.head :: y)) :=
+def to_bit : code := case one one zero
+@[simp] lemma to_bit_apply (n : ℕ) : to_bit.eval n = part.some (if n = 0 then 0 else 1) :=
 begin
-  simp only [cons, code.eval],
-  cases (f.eval impl bs) with d₁ v₁, by_cases h₁ : d₁, swap, { simp [h₁], }, simp only [h₁, part.mk_some],
-  cases (g.eval impl bs) with d₂ v₂, by_cases h₂ : d₂, swap, { simp [h₂], }, simp only [h₂, part.mk_some],
-  simp,
+  have := computability.encode_nat_nil_iff_zero n,
+  simp only [to_bit, code.eval],
+  rcases (encode_nat n) with _|_|_,
+  all_goals { intro, simp * at *, },
 end
 
-def snoc (f g : code ocl) : code ocl := appendᵒ ∘ {f, headᵒ ∘ g}
-def const_op (b : bool) : code ocl := if b = ff then ff'ᵒ else tt'ᵒ
-@[simp] lemma const_op_apply (b : bool) (bs : bitstring) :
-  (const_op b).eval impl bs = part.some [b] :=
-by cases b; simp [const_op]
 
-
-def bool_op (fn : bool → bool → bool) : code ocl :=
-(case 
-  (case (const_op $ fn ff ff) (const_op $ fn ff tt))
-  (case (const_op $ fn tt ff) (const_op $ fn tt tt)))
-
-lemma bool_op_apply (fn : bool → bool → bool) (b₁ b₂ : bool) (bs : list bool) :
-  (bool_op fn).eval impl (b₁ :: b₂ :: bs) = part.some [fn b₁ b₂] :=
-by cases b₁; cases b₂; simp [bool_op]
-
-def xor_code : code ocl := bool_op bxor
-
-def code_ite (c f g : code ocl) : code ocl :=
-  (case g f) ∘ (cons c idᵒ)
-
-@[simp] lemma code_ite_apply (c f g : code ocl) (bs : bitstring) :
-  (code_ite c f g).eval impl bs = (c.eval impl bs) >>= (λ r, if r.head = tt then f.eval impl bs else g.eval impl bs) :=
+def tail : code := snd ∘ (bit ff) ∘ (bit tt) ∘ (bit tt)
+@[simp] lemma tail_apply_bit1 (n : ℕ) : tail.eval (bit1 n) = part.some n :=
+by simp [tail, nat.bit, ← nat.mkpair'_one]
+@[simp] lemma tail_apply_bit0 (n : ℕ) : tail.eval (bit0 n) = part.some n :=
 begin
-  simp only [code_ite, code.eval, cons_apply],
-  cases (c.eval impl bs) with d₁ v₁, by_cases h₁ : d₁, swap, { simp [h₁], }, simp only [h₁, part.mk_some],
-  simp [← eq_ff_eq_not_eq_tt],
+  cases n;
+  simp [tail, nat.bit, nat.unpair', list.unpair, list.unpair', list.take_while, list.after],
 end
 
-def is_list_empty : code ocl := isemptyᵒ
-@[simp] lemma is_list_empty_apply {α : Type} [boolcodeable α] (ls : list α) :
-  is_list_empty.eval impl (encode ls) = part.some [ls.empty] :=
-by simp [is_list_empty, boolcodeable.list_encode_empty_iff]
-
-def list_head : code ocl := fstᵒ
-@[simp] lemma list_head_apply {α : Type} [boolcodeable α] (x : α) (xs : list α) :
-  list_head.eval impl (encode $ x :: xs) = part.some (encode x) :=
-by simp [list_head, boolcodeable.list_encode_def]
-
-def list_tail : code ocl := sndᵒ
-@[simp] lemma list_tail_apply {α : Type} [boolcodeable α] (x : α) (xs : list α) :
-  list_tail.eval impl (encode $ x :: xs) = part.some (encode xs) :=
-by simp [list_tail, boolcodeable.list_encode_def]
-
-def list_foldl_aux (step : code ocl /- (acc, hd) → acc -/) : code ocl :=
-let acc := fstᵒ,
-    hd := list_head ∘ sndᵒ,
-    tl := list_tail ∘ sndᵒ in
-code_ite (is_list_empty ∘ sndᵒ)
-  (append' ff'ᵒ acc) -- If it is empty, do not recurse further (append ff'ᵒ)
-  (append' tt'ᵒ {step ∘ {acc, hd}, tl}) -- Otherwise, append tt'ᵒ and do one step
-
-lemma list_foldl_aux_apply {α : Type} [boolcodeable α]
-  (step : code ocl) (acc : bitstring) (ls : list α) :
-  (list_foldl_aux step).eval impl (encode_tuple acc (encode ls)) = (ls.cases_on'
-    (part.some $ acc)
-    (λ hd tl, (step.eval impl $ encode_tuple acc (encode hd)).map (λ r, encode_tuple r (encode tl)))) 
-    .map (λ r, (bnot ls.empty) :: r) :=
-by cases ls; simp [list_foldl_aux, boolcodeable.encode_product_def]
-
-def list_foldl (step : code ocl) : code ocl := fix (list_foldl_aux step)
-
-lemma list_foldl_apply {α : Type} [boolcodeable α] (step : code ocl) (base : bitstring) (ls : list α) :
-  (list_foldl step).eval impl (encode_tuple base $ encode ls) =
-  ls.foldl (λ acc hd, acc >>= λ r, step.eval impl $ encode_tuple r (encode hd)) (part.some $ encode base) :=
+/-- Slight hack, uses details of the encoding of `pair` -/
+def cons_bit (f g : code) : code := (case (tail ∘ tail) (bit ff) zero) ∘ (pair (to_bit ∘ f) g)
+@[simp] lemma cons_bit_apply (f g : code) (n : ℕ) :
+  (cons_bit f g).eval n = f.eval n >>= (λ r, (g.eval n).map (if r = 0 then bit0 else bit1)) :=
 begin
-  induction ls with hd tl ih generalizing base,
-  { simp [list_foldl, part.eq_some_iff], apply pfun.fix_stop, rw list_foldl_aux_apply, simp, },
-  simp [list_foldl] at ⊢ ih,
-  rw pfun.fix_iterate' _ ((step.eval impl $ encode_tuple base (encode hd)).map (λ r, encode_tuple r (encode tl))),
-  { simp [ih], clear ih,
-    cases (step.eval impl $ encode_tuple base (encode hd)) with d₁ v₁, by_cases h₁ : d₁, swap, { simp [h₁], }, simp only [h₁, part.mk_some],
-    simp, },
-  clear ih, simp [list_foldl_aux_apply],
-  cases (step.eval impl $ encode_tuple base (encode hd)) with d₁ v₁, by_cases h₁ : d₁, swap, { simp [h₁], }, simp only [h₁, part.mk_some],
-  simp,
+  simp only [cons_bit, code.eval],
+  cases (f.eval n) with d₁ v₁, by_cases h₁ : d₁, swap, { simp [h₁], }, simp only [h₁, part.mk_some],
+  cases (g.eval n) with d₂ v₂, by_cases h₂ : d₂, swap, { simp [h₂], }, simp only [h₂, part.mk_some],
+  cases v₁ h₁,
+  { simp [nat.mkpair'_zero, nat.bit], },
+  { simp [nat.mkpair'_one, nat.bit], }
 end
 
-lemma list_foldl_apply' {α β : Type} [boolcodeable α] [boolcodeable β] (step : α → β → α) {step_cd : code ocl} (base : α) (ls : list β)
-  (hstep : ∀ (a : α) (b : β), step_cd.eval impl (encode (a, b)) = part.some (encode $ step a b)) :
-  (list_foldl step_cd).eval impl (encode (base, ls)) = part.some (encode (ls.foldl step base)) :=
+protected def code.ite (c f g : code) : code :=
+(case f g f) ∘ (cons_bit c code.id)
+@[simp] lemma code_ite_apply (c f g : code) (n : ℕ) :
+  (code.ite c f g).eval n = (c.eval n) >>= λ r, if r = 0 then f.eval n else g.eval n :=
 begin
-  simp [boolcodeable.encode_product_def, list_foldl_apply],
-  induction ls with hd tl ih generalizing base, { simp, }, 
-  simp [← boolcodeable.encode_product_def, hstep, ih],
+  simp only [code.ite, code.eval, cons_bit_apply, id_apply],
+  cases (c.eval n) with d₁ v₁, by_cases h₁ : d₁, swap, { simp [h₁], }, simp only [h₁, part.mk_some],
+  cases v₁ h₁,
+  { cases n; simp, }, simp,
 end
 
-def list_cons : code ocl := idᵒ
-@[simp] lemma list_cons_apply {α : Type} [boolcodeable α] (hd : α) (tl : list α) :
-  list_cons.eval impl (encode (hd, tl)) = part.some (encode (hd :: tl)) := rfl
-
-/-- TODO: let's make a prop `is_polynomial` which is true iff a function has *some implementation*
-  that is polynomial-time. This is a lot easier to think about, since we don't constantly have to deal
-  with encodings. Then, we can make a tactic like `continuity` for polynomial time functions.
-  
-  What we want to write here is
-  `reverse = λ x : list α, x.foldl (λ acc hd, hd :: acc) []`
-  and have lean automatically translate into the existence of something like this. -/
-def reverse : code ocl := list_foldl (list_cons ∘ {sndᵒ, fstᵒ}) ∘ {nil, idᵒ}
-lemma reverse_apply {α : Type} [boolcodeable α] (ls : list α) :
-  reverse.eval impl (encode ls) = part.some (encode (ls.reverse)) :=
-begin
-  simp [reverse],
-  have : encode (@list.nil bool, encode ls) = encode (@list.nil α, ls) := rfl, rw this, clear this,
-  rw list_foldl_apply' (λ acc hd, hd :: acc),
-  { congr, exact list.foldl_of_cons ls, },
-  intros a b,
-  simp [boolcodeable.encode_product_def],
-  rw ← boolcodeable.encode_product_def,
-  simp,
 end
 
-/- TODO: figure out why encoding/decoding nat's is somewhat slow -/
-#eval decode ℕ ((list_foldl addᵒ).eval impl $ encode (0, [0, 1, 5, 100])).unwrap
-end
