src/old/time_bound.lean
@@ -1,0 +1,74 @@
+import code
+import frespects_pfun
+
+/-! This code is adapted from Bolton Bailey's PR: https://github.com/leanprover-community/mathlib/pull/11046 -/
+
+open boolcodeable (encode decode)
+
+local attribute [reducible] bitstring
+
+def time {ι : Type} (impl : ι → bitstring → bitstring) : code ι → bitstring →. ℕ
+| (code.oracle i) := λ b, pure 1
+| (code.pair c₁ c₂) := λ v, (+1) <$> (time c₁ v) + (time c₂ v)
+| (code.comp c₁ c₂) := λ v, (+1) <$> (time c₂ v) + (c₂.eval impl v >>= time c₁)
+| (code.case c₁ c₂) := λ v, (+1) <$> (if v.head = ff then time c₁ v.tail else time c₂ v.tail)
+| (code.fix f) := λ v₀, (@pfun.fix (bitstring × ℕ) ℕ $ 
+  λ vt, (time f vt.1) >>= λ t',
+    (f.eval impl vt.1).map (λ v' : bitstring,
+      if v'.head = ff then sum.inl (vt.2+t')
+      else sum.inr (v'.tail, vt.2+t'))
+  ) (v₀, 0)
+
+variables {ι : Type} (impl : ι → bitstring → bitstring)
+
+lemma time_dom_iff_eval_dom (c : code ι) (b : bitstring) : (time impl c b).dom ↔ (c.eval impl b).dom :=
+begin
+  induction c generalizing b,
+  case code.oracle { simp [time], refl, },
+  case code.pair : c₁ c₂ c₁ih c₂ih { simp only [time, code.eval, (+), (<*>)], simp [c₁ih, c₂ih], },
+  case code.comp : c₁ c₂ c₁ih c₂ih { simp only [time, code.eval, (+), (<*>)], simp [c₁ih, c₂ih], tauto, },
+  case code.case : c₁ c₂ c₁ih c₂ih { simp only [time, code.eval], split_ifs; simp [c₁ih, c₂ih], },
+  case code.fix : f ih
+  { simp only [time, code.eval], refine pfun.eq_dom_of_frespects_once prod.fst _ _,
+    intro a, split,
+    { simp [ih], }, split,
+    { intro a',
+      simp only [part.bind_eq_bind, part.mem_bind_iff, part.mem_map_iff, exists_prop, forall_exists_index, and_imp],
+      intros n hn e he h, use e, refine ⟨he, _⟩,
+      split_ifs at h, { contradiction, },
+      rw ← h, split_ifs; refl,  },
+    simp only [part.bind_eq_bind, part.mem_bind_iff, part.mem_map_iff, exists_prop, forall_exists_index, and_imp],
+    intros n₁ n₂ hn₂ b hb h,
+    refine ⟨b.tail, b, hb, _⟩,
+    split_ifs at h ⊢, { refl, }, { contradiction, }, }
+end
+
+variables (c : code ι) (bound : ℕ → ℕ)
+def time_bound : Prop :=
+∀ (b : bitstring) (l : ℕ), b.sizeof ≤ l → ∃ t ∈ time impl c b, t ≤ bound l
+
+variables {impl c bound}
+lemma total_of_time_bound (H : time_bound impl c bound)
+  (b : bitstring) : (c.eval impl b).dom :=
+begin
+  rw ← time_dom_iff_eval_dom,
+  obtain ⟨n, t, _⟩ := H b b.sizeof (by refl),
+  rw part.dom_iff_mem, use n, assumption,
+end
+
+lemma time_bound_oracle (i : ι) :
+  time_bound impl (code.oracle i) 1 :=
+by { intros _ _ _, refine ⟨1, _, (by refl)⟩, simp [time], }
+
+
+lemma time_bound_pair (c₁ c₂ : code ι) {b₁ b₂ : ℕ → ℕ} (hb₁ : time_bound impl c₁ b₁) (hb₂ : time_bound impl c₂ b₂) :
+  time_bound impl (code.pair c₁ c₂) (λ n, b₁ n + b₂ n + 1) :=
+begin
+  intros b l hb, simp only [time],
+  obtain ⟨t₁, ht₁, t₁_le⟩ := hb₁ b l hb,
+  obtain ⟨t₂, ht₂, t₂_le⟩ := hb₂ b l hb,
+  use t₁ + t₂ + 1, split, swap, { linarith, },
+  simp only [part.eq_some_iff.mpr ht₁, part.eq_some_iff.mpr ht₂, (+), (<*>)], simp, ring,
+end
+
+
